Rename Mem2 -> Mem1 and others; all compiles!

mem/Mem1.v
@@ -8,14 +8,11 @@ Require Import Skeleton.
 Require Import PCM.
 Require Import HoareDef.
 Require Import TODOYJ.
+Require Import Logic.
 
 Generalizable Variables E R A B C X Y Σ.
 
 Set Implicit Arguments.
-
-
-
-
 
 
 
@@ -27,7 +24,7 @@ Compute (URA.car).
 Section PROOF.
   Context `{@GRA.inG memRA Σ}.
 
-  Definition _points_to (loc: block * Z) (vs: list val): Mem1._memRA :=
+  Definition _points_to (loc: block * Z) (vs: list val): _memRA :=
     let (b, ofs) := loc in
     (fun _b _ofs => if (dec _b b) && ((ofs <=? _ofs) && (_ofs <? (ofs + Z.of_nat (List.length vs))))%Z
                     then (List.nth_error vs (Z.to_nat (_ofs - ofs))) else ε)
@@ -109,51 +106,49 @@ Notation "loc |-> vs" := (points_to loc vs) (at level 20).
 
 
 
+
 Section PROOF.
   Context `{@GRA.inG memRA Σ}.
   Let GURA: URA.t := GRA.to_URA Σ.
   Local Existing Instance GURA.
 
   Let alloc_spec: fspec := (mk_simple "Mem"
-                                      (fun sz varg o _ => varg = [Vint (Z.of_nat sz)]↑ /\ o = ord_pure 1)
-                                      (fun sz vret rret =>
-                                         exists b, vret = (Vptr b 0)↑ /\
-                                                   rret = GRA.embed ((b, 0%Z) |-> (List.repeat (Vint 0) sz)))).
+                                      (fun sz varg o => ⌜varg = [Vint (Z.of_nat sz)]↑ /\ o = ord_pure 1⌝)
+                                      (fun sz vret => Exists b, ⌜vret = (Vptr b 0)↑⌝ **
+                                                   Own(GRA.embed ((b, 0%Z) |-> (List.repeat (Vint 0) sz))))).
 
   Let free_spec: fspec := (mk_simple "Mem"
-                                     (fun '(b, ofs) varg o rarg => exists v, varg = ([Vptr b ofs])↑ /\
-                                                                             rarg = GRA.embed ((b, ofs) |-> [v]) /\
-                                                                             o = ord_pure 1)
+                                     (fun '(b, ofs) varg o => Exists v, ⌜varg = ([Vptr b ofs])↑⌝ **
+                                                                        Own(GRA.embed ((b, ofs) |-> [v])) **
+                                                                        ⌜o = ord_pure 1⌝)
                                      (top3)).
 
   Let load_spec: fspec := (mk_simple "Mem"
-                                     (fun '(b, ofs, v) varg o rarg => varg = ([Vptr b ofs])↑ /\
-                                                                      rarg = GRA.embed ((b, ofs) |-> [v]) /\
-                                                                      o = ord_pure 1)
-                                     (fun '(b, ofs, v) vret rret => rret = GRA.embed ((b, ofs) |-> [v]) /\ vret = v↑)).
+                                     (fun '(b, ofs, v) varg o => ⌜varg = ([Vptr b ofs])↑⌝ **
+                                                                      Own(GRA.embed ((b, ofs) |-> [v])) **
+                                                                      ⌜o = ord_pure 1⌝)
+                                     (fun '(b, ofs, v) vret => Own(GRA.embed ((b, ofs) |-> [v])) ** ⌜vret = v↑⌝)).
 
   Let store_spec: fspec := (mk_simple
                               "Mem"
-                              (fun '(b, ofs, v_new) varg o rarg => exists v_old,
-                                   varg = ([Vptr b ofs ; v_new])↑ /\ rarg = GRA.embed ((b, ofs) |-> [v_old]) /\ o = ord_pure 1)
-                              (fun '(b, ofs, v_new) _ rret => rret = GRA.embed ((b, ofs) |-> [v_new]))).
+                              (fun '(b, ofs, v_new) varg o => Exists v_old,
+                                   ⌜varg = ([Vptr b ofs ; v_new])↑⌝ ** Own(GRA.embed ((b, ofs) |-> [v_old])) ** ⌜o = ord_pure 1⌝)
+                              (fun '(b, ofs, v_new) _ => Own(GRA.embed ((b, ofs) |-> [v_new])))).
 
   Let cmp_spec: fspec :=
     (mk_simple
        "Mem"
-       (fun '(result, resource) varg o rarg =>
-          rarg = resource /\
-          ((exists b ofs v, varg = [Vptr b ofs; Vnullptr]↑ /\ rarg = GRA.embed ((b, ofs) |-> [v]) /\ result = false) \/
-           (exists b ofs v, varg = [Vnullptr; Vptr b ofs]↑ /\ rarg = GRA.embed ((b, ofs) |-> [v]) /\ result = false) \/
-           (exists b0 ofs0 v0 b1 ofs1 v1, varg = [Vptr b0 ofs0; Vptr b1 ofs1]↑ /\
-                                          rarg = GRA.embed ((b0, ofs0) |-> [v0]) ⋅ GRA.embed ((b1, ofs1) |-> [v1]) /\ result = false) \/
-           (exists b ofs v, varg = [Vptr b ofs; Vptr b  ofs]↑ /\ rarg = GRA.embed ((b, ofs) |-> [v]) /\ result = true) \/
-           (varg = [Vnullptr; Vnullptr]↑ /\ result = true)
-          ) /\
-          o = ord_pure 1
+       (fun '(result, resource) varg o =>
+          ((Exists b ofs v, ⌜varg = [Vptr b ofs; Vnullptr]↑⌝ ** ⌜resource = (GRA.embed ((b, ofs) |-> [v]))⌝ ** ⌜result = false⌝) ∨
+           (Exists b ofs v, ⌜varg = [Vnullptr; Vptr b ofs]↑⌝ ** ⌜resource = (GRA.embed ((b, ofs) |-> [v]))⌝ ** ⌜result = false⌝) ∨
+           (Exists b0 ofs0 v0 b1 ofs1 v1, ⌜varg = [Vptr b0 ofs0; Vptr b1 ofs1]↑⌝ **
+                     ⌜resource = (GRA.embed ((b0, ofs0) |-> [v0])) ⋅ (GRA.embed ((b1, ofs1) |-> [v1]))⌝ ** ⌜result = false⌝) ∨
+           (Exists b ofs v, ⌜varg = [Vptr b ofs; Vptr b  ofs]↑⌝ ** ⌜resource = (GRA.embed ((b, ofs) |-> [v]))⌝ ** ⌜result = true⌝) ∨
+           (⌜varg = [Vnullptr; Vnullptr]↑ /\ result = true⌝))
+            ** Own(resource)
+            ** ⌜o = ord_pure 1⌝
        )
-       (fun '(result, resource) vret rret =>
-          vret = (if result then Vint 1 else Vint 0)↑ /\ rret = resource)
+       (fun '(result, resource) vret => Own(resource) ** ⌜vret = (if result then Vint 1 else Vint 0)↑⌝)
     ).
 
   Definition MemStb: list (gname * fspec).
@@ -173,8 +168,7 @@ Section PROOF.
   Definition MemSem: ModSem.t := {|
     ModSem.fnsems := List.map (fun '(fn, fsb) => (fn, fun_to_tgt MemStb fn fsb)) MemSbtb;
     ModSem.initial_mrs :=
-      [("Mem", (GRA.embed (URA.black (M:=_memRA)
-                            (fun b ofs => if (b =? 0)%nat && (ofs =? 0)%Z then (Some Vundef) else ε)), tt↑))];
+      [("Mem", (GRA.embed (URA.black (M:=_memRA) ε), tt↑))];
   |}
   .
 
@@ -187,5 +181,4 @@ Section PROOF.
 End PROOF.
 Global Hint Unfold MemStb: stb.
 
-(* Opaque points_to. *)
 Global Opaque _points_to.
