examples/delayed_echo/Echo1.v
@@ -6,7 +6,7 @@ Require Import ModSem.
 Require Import Skeleton.
 Require Import PCM.
 Require Import HoareDef.
-Require Import Stack1 Client1 Mem2.
+Require Import Stack1 Client1 Mem1.
 Require Import TODOYJ.
 Require Import Logic.
 
