examples/delayed_echo/Stack1.v
@@ -7,7 +7,7 @@ Require Import Skeleton.
 Require Import PCM.
 Require Import HoareDef.
 Require Import Logic.
-Require Import Mem1 Mem2.
+Require Import Mem1.
 Require Import TODOYJ.
 
 Generalizable Variables E R A B C X Y Σ.
