mem/Mem01proof.v
@@ -16,7 +16,7 @@ From ExtLib Require Import
      Structures.Maps
      Data.Map.FMapAList.
 Require Import TODOYJ.
-Require Import HTactics.
+Require Import HTactics Logic YPM.
 
 Generalizable Variables E R A B C X Y.
 
@@ -57,342 +57,424 @@ Definition add_delta_to_black `{M: URA.t} (b: URA.auth_t) (w: URA.auth_t): URA.a
 (* "). *)
 (******** TODO: it works in emacs but fails in coqc -- try coq 8.13 and uncomment it ***********)
 
+Lemma repeat_nth_some
+      X (x: X) sz ofs
+      (IN: ofs < sz)
+  :
+    nth_error (repeat x sz) ofs = Some x
+.
+Proof.
+  ginduction sz; ii; ss.
+  - lia.
+  - destruct ofs; ss. exploit IHsz; et. lia.
+Qed.
 
+Lemma repeat_nth_none
+      X (x: X) sz ofs
+      (IN: ~(ofs < sz))
+  :
+    nth_error (repeat x sz) ofs = None
+.
+Proof.
+  generalize dependent ofs. induction sz; ii; ss.
+  - destruct ofs; ss.
+  - destruct ofs; ss. { lia. } hexploit (IHsz ofs); et. lia.
+Qed.
+
+Lemma repeat_nth
+      X (x: X) sz ofs
+  :
+    nth_error (repeat x sz) ofs = if (ofs <? sz) then Some x else None
+.
+Proof.
+  des_ifs.
+  - eapply repeat_nth_some; et. apply_all_once Nat.ltb_lt. ss.
+  - eapply repeat_nth_none; et. apply_all_once Nat.ltb_ge. lia.
+Qed.
+
+
+
+Section AUX.
+  Context {K: Type} `{M: URA.t}.
+  Let RA := URA.pointwise K M.
+
+  Lemma pw_extends (f0 f1: K -> M) (EXT: @URA.extends RA f0 f1): forall k, <<EXT: URA.extends (f0 k) (f1 k)>>.
+  Proof. ii. r in EXT. des. subst. ur. ss. eexists; et. Qed.
+  (* Lemma pw_unfold_wf (f: K -> M): (forall k, URA.wf (f k)) -> @URA.wf RA f. Proof. i. ss. Qed. *)
+
+  (* Lemma empty_wf: forall k, URA.wf ((@URA.unit RA) k). *)
+  (* Proof. ii; ss. eapply URA.wf_unit. Qed. *)
+
+  (* Lemma update_wf: forall `{Dec K} (f: @URA.car RA) k v (WF: URA.wf f) (WF: URA.wf v), URA.wf (update f k v: (@URA.car RA)). *)
+  (* Proof. ii. unfold update. des_ifs; ss. Qed. *)
+
+  Lemma lookup_wf: forall (f: @URA.car RA) k (WF: URA.wf f), URA.wf (f k).
+  Proof. ii; ss. rewrite URA.unfold_wf in WF. ss. Qed.
+
+End AUX.
+
+Section AUX.
+  Context `{Σ: GRA.t}.
+  Definition Univ {X: Type} (P: X -> iProp): iProp := fun r => forall x, P x r.
+End AUX.
+Notation "'Forall' x .. y , p" := (Univ (fun x => .. (Univ (fun y => p)) ..))
+                                    (at level 200, x binder, right associativity,
+                                     format "'[' 'Forall'  '/  ' x  ..  y ,  '/  ' p ']'").
+
+Ltac Ztac := all_once_fast ltac:(fun H => first[apply Z.leb_le in H|apply Z.ltb_lt in H|apply Z.leb_gt in H|apply Z.ltb_ge in H|idtac]).
+
+Lemma _points_to_hit: forall b ofs v, (_points_to (b, ofs) [v] b ofs) = (Some v).
+Proof. i. rewrite unfold_points_to. ss. des_ifs; bsimpl; des; des_sumbool; subst; Ztac; try lia. rewrite Z.sub_diag. ss. Qed.
+
+Lemma _points_to_miss: forall b ofs b' ofs' (MISS: b <> b' \/ ofs <> ofs') v, (_points_to (b, ofs) [v] b' ofs') = ε.
+Proof. i. rewrite unfold_points_to. ss. des_ifs; bsimpl; des; des_sumbool; subst; Ztac; try lia. Qed.
+
+Lemma dec_true: forall X `{Dec X} (x0 x1: X), x0 = x1 -> ((dec x0 x1): bool) = true.
+Proof. ii. subst. unfold dec. destruct H; ss. Qed.
+
+Lemma dec_false: forall X `{Dec X} (x0 x1: X), x0 <> x1 -> ((dec x0 x1): bool) = false.
+Proof. ii. subst. unfold dec. destruct H; ss. Qed.
+(* Lemma local_update_same *)
+(*       `{M: URA.t} *)
+(*       x0 y0 x1 y1 *)
+(*       (SAME: x0 ⋅ y0 = x1 ⋅ y1) *)
+(*   : *)
+(*     URA.local_update x0 y0 x1 y1 *)
+(* . *)
+(* Proof. *)
+(*   r. ii. des. subst. esplits; et. *)
+(*   - *)
+(* Qed. *)
 
 Section SIMMODSEM.
 
   Context `{Σ: GRA.t}.
-  Context `{@GRA.inG Mem1.memRA Σ} `{@GRA.inG (RA.excl Mem.t) Σ}.
+  Context `{@GRA.inG Mem1.memRA Σ}.
 
   Let W: Type := (alist mname (Σ * Any.t)) * (alist mname (Σ * Any.t)).
   (* Eval compute in (@RA.car (RA.excl Mem.t)). *)
   Eval compute in (@URA.car Mem1._memRA).
-  Inductive sim_loc: option val -> (option val + unit) -> Prop :=
-  | sim_loc_present v: sim_loc (Some v) (inl (Some v))
-  | sim_loc_absent: sim_loc None (inr tt)
+  Inductive sim_loc: option val -> URA.car (t:=(URA.Excl.t _)) -> Prop :=
+  | sim_loc_present v: sim_loc (Some v) (Some v)
+  | sim_loc_absent: sim_loc None ε
   .
 
   Let wf: W -> Prop :=
     fun '(mrps_src0, mrps_tgt0) =>
-      exists mem_src (mem_tgt: Mem.t),
-        (<<SRC: mrps_src0 = Maps.add "Mem" ((GRA.embed ((URA.black mem_src): URA.car (t:=Mem1.memRA))), tt↑) Maps.empty>>) /\
+      exists mr_src (mem_tgt: Mem.t),
+        (<<SRC: mrps_src0 = Maps.add "Mem" (mr_src, tt↑) Maps.empty>>) /\
         (<<TGT: mrps_tgt0 = Maps.add "Mem" (ε, mem_tgt↑) Maps.empty>>) /\
-        (<<SIM: forall b ofs, sim_loc ((mem_tgt.(Mem.cnts)) b ofs) (mem_src b ofs)>>)
+        (* (<<SIM: forall b ofs, sim_loc ((mem_tgt.(Mem.cnts)) b ofs) (mem_src b ofs)>>) *)
+        (* (<<SIM: forall b ofs v, (mem_tgt.(Mem.cnts) b ofs = Some v) -> iHyp (⌜True⌝) mem_src>>) *)
+        (* (<<SIM: iHyp (Forall b ofs v, ⌜mem_tgt.(Mem.cnts) b ofs = Some v⌝ -* Own (GRA.embed ((b, ofs) |-> [v]))) mem_src>>) *)
+        (<<SIM: iHyp (Exists mem_src, Own (GRA.embed ((URA.black mem_src): URA.car (t:=Mem1.memRA))) **
+                                          (* (Forall b ofs, ⌜~(b = 0 /\ ofs = 0%Z)⌝ -* *)
+                                          (*                  match mem_tgt.(Mem.cnts) b ofs with *)
+                                          (*                  | Some v => Own (GRA.embed ((b, ofs) |-> [v])) *)
+                                          (*                  | None => ⌜True⌝ *)
+                                          (*                  end) *)
+                                          (⌜forall b ofs, sim_loc ((mem_tgt.(Mem.cnts)) b ofs) (mem_src b ofs)⌝)
+                     ) mr_src>>) /\
+        (<<WFTGT: forall b ofs v, mem_tgt.(Mem.cnts) b ofs = Some v -> <<NB: b < mem_tgt.(Mem.nb)>> >>)
   .
-
-  Local Opaque points_to.
 
   Hint Resolve sim_itree_mon: paco.
 
+  (* Lemma just_wf `{M: RA.t}: forall (x: @RA.car M), RA.wf x -> @URA.wf (URA.of_RA.t M) (URA.of_RA.just x). *)
+  (* Proof. i; ss. Qed. *)
+
+  (* Opaque URA.of_RA.t. *)
+  (* Opaque URA.auth. *)
+  (* Opaque URA.pointwise. *)
   Opaque URA.unit.
 
   Theorem correct: ModSemPair.sim Mem1.MemSem Mem0.MemSem.
   Proof.
    econstructor 1 with (wf:=wf) (le:=top2); et; swap 2 3.
     { typeclasses eauto. }
-    { ss. esplits; ss; et. ii.
-      destruct (classic (b = 0%nat /\ ofs = 0%Z)).
-      - des. subst. ss. unfold update. des_ifs. econs.
-      - des_ifs; bsimpl; des; des_sumbool; ss; try rewrite Nat.eqb_neq in *; try rewrite Z.eqb_neq in *;
-          apply_all_once Nat.eqb_eq; apply_all_once Z.eqb_eq; subst; try lia.
-        + unfold update. des_ifs; econs; et.
-        + unfold update. des_ifs; econs; et.
+    { ss. esplits; ss; et. hexploit gwf_dummy; i. iRefresh.
+      eexists; iRefresh. iSplitP; ss.
+      { eexists. rewrite URA.unit_id. refl. }
+      ii. econs.
     }
 
     econs; ss.
-    { unfold allocF. init. harg_tac. des; clarify.
-      unfold interp_hCallE_tgt, APC. steps. anytac. ss.
-      steps. force_l. exists 0. steps. force_l. exists (Vptr (Mem.nb mem_tgt) 0).
-      set (blk := (Mem.nb mem_tgt)). rename x into sz.
-      assert(WFA: forall ofs, mem_src (Mem.nb mem_tgt) ofs = inr tt).
-      { i.
-        destruct (mem_src (Mem.nb mem_tgt) ofs) eqn:A; cycle 1.
-        { des_u; ss. }
-        destruct o.
-        - admit "ez - add tgt wf".
-        - admit "ez - inl None is boom in RA.excl".
+    { unfold allocF. init.
+      harg_tac. des_ifs_safe. des. repeat rewrite URA.unit_idl in *. repeat rewrite URA.unit_id in *.
+      iRefresh. iPure PRE. des. clarify. apply Any.upcast_inj in PRE. des; clarify.
+      steps. rewrite Any.upcast_downcast in *. steps.
+      do 2 iDestruct SIM. iPure A.
+      set (blk := (Mem.nb mem_tgt)). rename x into sz. rename x0 into mem_src0.
+
+      unfold interp_hCallE_tgt, APC. steps. (********** TODO: never unfold it, make a lemma ******************)
+      force_l. exists 0. steps.
+
+      eapply own_upd in SIM; cycle 1; [|rewrite intro_iHyp in SIM; iMod SIM].
+      { eapply GRA.embed_updatable.
+        eapply URA.auth_alloc2.
+        instantiate (1:=(_points_to (blk, 0%Z) (repeat (Vint 0) sz))).
+        (* instantiate (1:=(fun _b _ofs => if (dec _b blk) && ((0 <=? _ofs) && (_ofs <? Z.of_nat sz))%Z then inl (Some (Vint 0)) else inr tt)). *)
+        iOwnWf SIM. iRefresh.
+        clear - WF WFTGT A.
+        ss. do 2 ur. ii. rewrite unfold_points_to. des_ifs.
+         - bsimpl. des. des_sumbool. subst. hexploit (A blk k0); et. intro T. inv T; [|eq_closure_tac].
+           + exploit WFTGT; et. i; des. lia.
+           + rewrite URA.unit_idl. Ztac. rewrite repeat_length in *. rewrite Z.sub_0_r. rewrite repeat_nth_some; [|lia]. ur. ss.
+         - rewrite URA.unit_id. do 2 eapply lookup_wf. eapply GRA.embed_wf in WF. des. ur in WF. admit "black wf".
       }
-      hret_tac (GRA.embed (add_delta_to_black
-                               (URA.black (mem_src: URA.car (t:=Mem1._memRA)))
-                               (points_to (blk, 0%Z) (repeat (Vint 0) sz)): URA.car (t:=Mem1.memRA)))
-      (GRA.embed ((blk, 0%Z) |-> (List.repeat (Vint 0) sz))).
-      { Local Opaque URA.add. etrans.
-        { eapply URA.extends_updatable. eexists; et. }
-        erewrite GRA.embed_add. eapply GRA.embed_updatable.
-        ss. des_ifs. eapply URA.auth_alloc2.
-        eapply URA.wf_mon in VALID.
-        eapply GRA.embed_wf in VALID. des.
-        clear - VALID WFA Heq SIM.
-        Local Transparent URA.add points_to.
-        ss. des. unfold URA.white in Heq. clarify.
-        ii. des_ifs; ss.
-        - bsimpl; des; des_sumbool; clarify.
-          exploit WFA; et. intro A. rewrite A in *; ss.
-        - specialize (VALID0 k k0). bsimpl; des; des_sumbool; clarify; des_ifs.
-        - specialize (VALID0 k k0). bsimpl; des; des_sumbool; clarify; des_ifs.
-          apply_all_once Z.leb_le. apply_all_once Z.ltb_lt.
-          intro A. apply nth_error_None in A. rewrite repeat_length in *.
-          apply inj_le in A. rewrite Z2Nat.id in A; cycle 1.
-          { lia. }
-          lia.
-          Local Opaque URA.add points_to.
-      }
-      { esplits; ss. }
-      { Local Opaque URA.wf.
-        Local Opaque URA.add points_to.
+      rewrite <- GRA.embed_add in SIM. rewrite own_sep in SIM. iDestruct SIM.
+
+      force_l. eexists. hret_tac SIM A0.
+      - split; [|refl]; iRefresh. eexists; iRefresh. iSplitP; ss.
+      - cbn. esplits; et.
+        + eexists; iRefresh. iSplitL SIM; et. ii.
+          destruct (mem_tgt.(Mem.cnts) blk ofs) eqn:T.
+          { exfalso. exploit WFTGT; et. i; des. lia. }
+          ss. do 2 ur.
+          exploit A; et. rewrite T. intro U. inv U. rewrite unfold_points_to. ss. rewrite repeat_length.
+          destruct (dec b blk); subst; ss.
+          * unfold update. des_ifs_safe. rewrite <- H0. rewrite URA.unit_idl. des_ifs.
+            { rewrite Z.sub_0_r. bsimpl. des. Ztac. rewrite repeat_nth_some; try lia. econs. }
+            { econs. }
+          * rewrite URA.unit_id. unfold update. des_ifs.
+        + clear - WFTGT. i. ss. unfold update in *. des_ifs. exploit WFTGT; et.
+    }
+    econs; ss.
+    { unfold freeF. init.
+      harg_tac. des_ifs_safe. des. repeat rewrite URA.unit_idl in *. repeat rewrite URA.unit_id in *.
+      iRefresh. do 3 iDestruct PRE. iPure PRE. iPure A. clarify. apply Any.upcast_inj in PRE. des; clarify.
+      do 2 iDestruct SIM. iPure A.
+      steps. rewrite Any.upcast_downcast in *. steps.
+
+      unfold interp_hCallE_tgt, APC. steps. (********** TODO: never unfold it, make a lemma ******************)
+      force_l. exists 0. steps.
+
+      rename n into b. rename z into ofs. rename x0 into mem_src0. rename x into v.
+      iMerge SIM A0. rewrite <- own_sep in SIM. rewrite GRA.embed_add in SIM.
+      iOwnWf SIM. eapply GRA.embed_wf in WF; des.
+      assert(HIT: mem_src0 b ofs = (Some v)).
+      { clear - WF.
         Local Transparent points_to.
-        ss. esplits; ss. i. ss.
-        destruct (dec b blk).
-        + subst. unfold blk. unfold update. des_ifs_safe. ss.
-          des_ifs.
-          * bsimpl; des; try rewrite Z.leb_le in *; try rewrite Z.ltb_lt in *.
-            Local Transparent URA.add.
-            s.
-            Local Opaque URA.add.
-            des_ifs; bsimpl; des; des_sumbool; ss; clarify; try rewrite Z.leb_le in *; try rewrite Z.ltb_lt in *;
-              try rewrite Z.leb_gt in *; try rewrite Z.ltb_ge in *; try lia; et.
-            { exploit WFA; et. intro A. rewrite A in *; ss. }
-            { exploit WFA; et. intro A. rewrite A in *; ss. }
-            { rewrite Z.sub_0_r.
-              destruct (nth_error (repeat (Vint 0) sz) (Z.to_nat ofs)) eqn:U.
-              - eapply nth_error_In in U. eapply repeat_spec in U. subst. econs; et.
-              - eapply nth_error_None in U. lia.
-            }
-            { rewrite repeat_length in *. lia. }
-          * Local Transparent URA.add.
-            s.
-            Local Opaque URA.add.
-            des_ifs; bsimpl; des; des_sumbool; ss; clarify; try rewrite Z.leb_le in *; try rewrite Z.ltb_lt in *;
-              try rewrite Z.leb_gt in *; try rewrite Z.ltb_ge in *; try lia; et;
-                try (by exploit WFA; et; intro A; rewrite A in *; ss).
-            { rewrite Z.sub_0_r. rewrite repeat_length in *. lia. }
-            { econs; eauto. }
-            { econs; eauto. }
-        + Local Transparent URA.add.
-          ss.
-          hexploit (SIM b ofs); et. intro A. inv A.
-          {
-            des_ifs; bsimpl; des; des_sumbool; clarify.
-            - unfold update. des_ifs. rewrite <- H1. econs.
-            - unfold update. des_ifs. rewrite <- H1. econs.
-            - unfold update. des_ifs. rewrite <- H1. econs.
-          }
-          {
-            des_ifs; bsimpl; des; des_sumbool; clarify.
-            - unfold update. des_ifs. rewrite <- H1. econs.
-            - unfold update. des_ifs. rewrite <- H1. econs.
-            - unfold update. des_ifs. rewrite <- H1. econs.
-          }
+        eapply URA.auth_included in WF. des. eapply pw_extends in WF. eapply pw_extends in WF.
+        rewrite _points_to_hit in WF.
+        admit "ez".
       }
-    }
-    econs; ss.
-    { unfold freeF. init. harg_tac. des; clarify.
-      unfold interp_hCallE_tgt, APC. steps. anytac. ss.
-      steps. force_l. exists 0. steps. anytac. ss. steps.
-      rewrite URA.unit_idl in *. rewrite GRA.embed_add in *. eapply GRA.embed_wf in VALID. des.
-      rename n into b. rename z into ofs.
-      assert(A: mem_src b ofs = inl (Some v)).
-      { Local Transparent URA.wf.
-        ss.
-        Local Transparent URA.add.
-        ss. des_ifs. des. specialize (VALID0 b ofs).
-        Local Transparent URA.add.
-        clear SIM.
-        Local Transparent URA.unit.
-        ss. clarify. rr in VALID. des. clarify. ss.
-        des_ifs;
-          bsimpl; des; des_sumbool; ss;
-          repeat des_u;
-          clear_tac;
-          try rewrite Z.leb_le in *; try rewrite Z.leb_gt in *; try rewrite Z.ltb_lt in *; try rewrite Z.ltb_ge in *;
-          try rewrite Z.sub_diag in *;
-          try lia; ss.
-        Local Opaque URA.wf URA.add URA.unit.
+      set (mem_src1 := fun _b _ofs => if dec _b b && dec _ofs ofs then (ε: URA.car (t:=URA.Excl.t _)) else mem_src0 _b _ofs).
+      assert(WF': URA.wf (mem_src1: URA.car (t:=Mem1._memRA))).
+      { clear - WF. unfold mem_src1. do 2 ur. ii. eapply URA.wf_mon in WF. ur in WF. des.
+        des_ifs; et.
+        - rp; [eapply URA.wf_unit|ss].
+        - do 2 eapply lookup_wf; et.
       }
-
-      set (mem_src' := fun _b _ofs => if dec _b b && dec _ofs ofs then inr () else mem_src _b _ofs).
-      assert(WF': URA.wf (mem_src': URA.car (t:=Mem1._memRA))).
-      { Local Transparent URA.add URA.wf.
-        ss. ii. des_ifs.
-        ss. clarify.
-        subst mem_src'. ss. des_ifs. des. specialize (VALID0 k k0). bsimpl. des; des_sumbool; des_ifs.
-        Local Opaque URA.wf URA.add.
-      }
-      hexploit (SIM b ofs); et. intro B. rewrite A in *. inv B.
+      hexploit (A b ofs); et. rewrite HIT. intro B. inv B.
       force_r.
-      { exfalso. unfold Mem.free in *. des_ifs. }
-      rename t into mem_tgt'.
-      assert(SIM': forall b ofs, sim_loc (Mem.cnts mem_tgt' b ofs) (mem_src' b ofs)).
-      { i.
-        unfold Mem.free in _UNWRAPU. des_ifs. ss.
-        subst mem_src'. ss.
-        destruct (classic (b = b0 /\ ofs = ofs0)); des; clarify.
-        - destruct H0; clarify. (**** TODO: FIX ****) unfold update. des_ifs. econs.
-        - des_ifs.
-          { Psimpl. bsimpl; des; des_sumbool; ss; clarify. destruct H0; ss. destruct H1; ss. (**** TODO: FIX ****)}
-          replace (update (Mem.cnts mem_tgt) b (update (Mem.cnts mem_tgt b) ofs None) b0 ofs0) with
-              (Mem.cnts mem_tgt b0 ofs0); cycle 1.
-          { unfold update. des_ifs. Psimpl. des_ifs; bsimpl; des; des_sumbool; ss; clarify. }
-          et.
-      }
-      force_l. esplits. steps.
-      hret_tac (GRA.embed (URA.black (mem_src': URA.car (t:=Mem1._memRA)))) (@URA.unit Σ).
-      { rewrite URA.unit_id.
-        rewrite ! GRA.embed_add. apply GRA.embed_updatable.
-        apply URA.auth_dealloc.
-        clear - WF' VALID.
+      { unfold Mem.free in *. des_ifs. }
+      rename mem_tgt into mem_tgt0. rename t into mem_tgt1.
+
+      eapply own_upd in SIM; cycle 1; [|rewrite intro_iHyp in SIM; iMod SIM].
+      { eapply GRA.embed_updatable.
+        Local Transparent points_to.
+        eapply URA.auth_dealloc.
+        instantiate (1:=mem_src1).
+        clear - WF'.
+
         r. i. rewrite URA.unit_idl.
+        Local Opaque Mem1._memRA.
         ss. destruct H; clear H. (*** coq bug; des infloops ***) des. clarify.
         esplits; et.
+        Local Transparent Mem1._memRA.
+        unfold mem_src1. ss.
         apply func_ext. intro _b. apply func_ext. intro _ofs.
-        destruct (classic (b = _b /\ ofs = _ofs)).
-        - destruct H; clear H. clarify.
-          subst mem_src'. ss. des_ifs; bsimpl; des; des_sumbool; clarify.
+        des_ifs.
+        - bsimpl; des; des_sumbool; subst.
+          subst mem_src1. do 2 ur in WF'. do 2 spc WF'. des_ifs; bsimpl; des; des_sumbool; ss.
           clear - H0.
-          Local Transparent URA.wf.
-          Local Transparent URA.add.
-          specialize (H0 _b _ofs). ss.
-          des_ifs; bsimpl; des; des_sumbool;
-            try rewrite Z.leb_le in *; try rewrite Z.leb_gt in *; try rewrite Z.ltb_lt in *; try rewrite Z.ltb_ge in *;
-              try rewrite Z.sub_diag in *;
-              try lia; ss.
-          des_u. ss.
-        - Psimpl.
-          subst mem_src'. s.
-          des_ifs; bsimpl; des; des_sumbool;
-            try rewrite Z.leb_le in *; try rewrite Z.leb_gt in *; try rewrite Z.ltb_lt in *; try rewrite Z.ltb_ge in *;
-              try rewrite Z.sub_diag in *;
-              try lia; ss.
-          Local Opaque URA.wf.
-          Local Opaque URA.add.
+          do 2 ur in H0.
+          specialize (H0 b ofs).
+          des_ifs; bsimpl; des; des_sumbool; Ztac; try lia. try rewrite Z.sub_diag in *; ss.
+          admit "ez".
+        - rewrite unfold_points_to in *. do 2 ur. do 2 ur in H0.
+          bsimpl. des_ifs; bsimpl; des; des_sumbool; subst; Ztac; try lia; try rewrite URA.unit_idl; try refl.
       }
-      { split; ss. }
-      { unfold wf. esplits; eauto. }
+      steps. iRefresh. force_l. eexists. hret_tac SIM (@URA.unit Σ).
+      { split; [|refl]. ss. }
+      { ss. esplits; ss; et.
+        - eexists mem_src1; iRefresh. iSplitP; ss. ii.
+          { unfold Mem.free in _UNWRAPU. des_ifs. ss.
+            subst mem_src1. ss.
+            destruct (classic (b = b0 /\ ofs = ofs0)); des; clarify.
+            - unfold update. des_ifs. econs.
+            - des_ifs.
+              { Psimpl. bsimpl; des; des_sumbool; ss; clarify. }
+              replace (update (Mem.cnts mem_tgt0) b (update (Mem.cnts mem_tgt0 b) ofs None) b0 ofs0) with
+                  (Mem.cnts mem_tgt0 b0 ofs0); cycle 1.
+              { unfold update. des_ifs. Psimpl. des_ifs; bsimpl; des; des_sumbool; ss; clarify. }
+              et.
+          }
+        - clear - _UNWRAPU WFTGT. ii. unfold Mem.free in *. des_ifs. ss.
+          unfold update in *. des_ifs; eapply WFTGT; et.
+      }
     }
     econs; ss.
-    { unfold loadF. init. harg_tac. des; clarify.
-      unfold interp_hCallE_tgt, APC. steps. anytac. ss.
-      steps. force_l. exists 0. steps. anytac. ss. steps.
-      rewrite URA.unit_idl in *. rewrite GRA.embed_add in *. apply_all_once GRA.embed_wf. des.
-      rename n into b. rename z into ofs.
-      assert(T: mem_src b ofs = inl (Some v)).
-      { Local Transparent points_to URA.add URA.wf URA.unit.
-        clear - VALID.
-        ss. des. do 2 spc VALID0. rr in VALID. des. ss.
-        des_ifs; bsimpl; des; des_sumbool; ss;
-          try rewrite Z.leb_le in *; try rewrite Z.leb_gt in *; try rewrite Z.ltb_lt in *; try rewrite Z.ltb_ge in *;
-            try rewrite Z.sub_diag in *; try lia; ss.
-        Local Opaque points_to URA.add URA.wf URA.unit.
+    { unfold loadF. init.
+      harg_tac. des_ifs_safe. des. repeat rewrite URA.unit_idl in *. repeat rewrite URA.unit_id in *.
+      iRefresh. do 2 iDestruct PRE. iPure PRE. iPure A. clarify. apply Any.upcast_inj in PRE. des; clarify.
+      do 2 iDestruct SIM. iPure A.
+      steps. rewrite Any.upcast_downcast in *. steps.
+
+      unfold interp_hCallE_tgt, APC. steps. (********** TODO: never unfold it, make a lemma ******************)
+      force_l. exists 0. steps.
+      rename n into b. rename z into ofs. rename x into mem_src0.
+      iMerge SIM A0. rewrite <- own_sep in SIM. rewrite GRA.embed_add in SIM. iOwnWf SIM.
+      assert(T: mem_src0 b ofs = (Some v)).
+      { clear - WF.
+        apply GRA.embed_wf in WF. des; ss. eapply URA.auth_included in WF. des.
+        eapply pw_extends in WF. eapply pw_extends in WF. rewrite _points_to_hit in WF.
+        des; ss.
+        admit "ez".
       }
-      exploit SIM; et. intro U. rewrite T in U. inv U; ss. unfold Mem.load.
+      exploit A; et. intro U. rewrite T in U. inv U; ss. unfold Mem.load.
+      rewrite <- GRA.embed_add in SIM. rewrite own_sep in SIM. iDestruct SIM.
       force_r; ss. clarify. steps. force_l. esplits.
-      hret_tac (GRA.embed (URA.black (mem_src: URA.car (t:=Mem1._memRA)))) (GRA.embed ((b, ofs) |-> [v0])); ss.
-      esplits; eauto.
+      hret_tac SIM A0.
+      { split; [|refl]; iRefresh. iSplitP; ss. }
+      { ss. esplits; eauto. eexists; iRefresh. iSplitP; ss; et. }
     }
     econs; ss.
-    { unfold storeF. init. harg_tac. des; clarify.
-      unfold interp_hCallE_tgt, APC. steps. anytac. ss.
-      steps. force_l. exists 0. steps. anytac. ss. steps.
-      rewrite URA.unit_idl in *. rewrite GRA.embed_add in *. apply_all_once GRA.embed_wf. des.
-      rename n into b. rename z into ofs.
-      set (mem_src' := fun _b _ofs => if dec _b b && dec _ofs ofs then inl (Some v) else mem_src _b _ofs).
-      assert(WF0: URA.wf (mem_src': URA.car (t:=Mem1._memRA))).
-      { Local Transparent URA.wf.
-        clear - VALID. apply URA.wf_mon in VALID. ss. des.
-        ii. specialize (VALID0 k k0). des_ifs_safe. unfold mem_src' in *. des_ifs.
-        Local Opaque URA.wf.
+    { unfold storeF. init.
+      harg_tac. des_ifs_safe. des. repeat rewrite URA.unit_idl in *. repeat rewrite URA.unit_id in *.
+      iRefresh. do 3 iDestruct PRE. iPure PRE. iPure A. clarify. apply Any.upcast_inj in PRE. des; clarify.
+      do 2 iDestruct SIM. iPure A.
+      steps. rewrite Any.upcast_downcast in *. steps.
+
+      unfold interp_hCallE_tgt, APC. steps. (********** TODO: never unfold it, make a lemma ******************)
+      force_l. exists 0. steps.
+      rename n into b. rename z into ofs. rename x0 into mem_src0. rename x into v0. rename v into v1.
+      iMerge SIM A0. rewrite <- own_sep in SIM. rewrite GRA.embed_add in SIM. iOwnWf SIM.
+      assert(T: mem_src0 b ofs = (Some v0)).
+      { clear - WF.
+        apply GRA.embed_wf in WF. des; ss. eapply URA.auth_included in WF. des.
+        eapply pw_extends in WF. eapply pw_extends in WF. rewrite _points_to_hit in WF.
+        des; ss.
+        admit "ez".
       }
-      assert(U: mem_src b ofs = inl (Some v_old)).
-      { Local Transparent URA.add GRA.to_URA points_to URA.wf URA.unit.
-        clear - VALID. ss. des. specialize (VALID0 b ofs). r in VALID. des; clarify. ss.
-        des_ifs; bsimpl; des; des_sumbool; ss; subst;
-          try rewrite Z.leb_le in *; try rewrite Z.leb_gt in *; try rewrite Z.ltb_lt in *; try rewrite Z.ltb_ge in *;
-            try rewrite Z.sub_diag in *; try lia; ss.
-        Local Opaque URA.add GRA.to_URA points_to URA.wf URA.unit.
+      exploit A; et. intro U. rewrite T in U. inv U; ss. unfold Mem.store. des_ifs. steps.
+      set (mem_src1 := fun _b _ofs => if dec _b b && dec _ofs ofs then (Some v1: URA.car (t:=URA.Excl.t _)) else mem_src0 _b _ofs).
+      eapply GRA.embed_wf in WF; des.
+      assert(WF': URA.wf (mem_src1: URA.car (t:=Mem1._memRA))).
+      { clear - WF. unfold mem_src1. do 2 ur. ii. eapply URA.wf_mon in WF. ur in WF. des.
+        des_ifs; et.
+        - bsimpl; des; des_sumbool; subst. admit "ez".
+        - do 2 eapply lookup_wf; et.
       }
-      hexploit SIM; et. intro V. rewrite U in V. inv V; ss. unfold Mem.store. rewrite <- H1. steps.
-      force_l. esplit.
-      hret_tac (GRA.embed (URA.black (mem_src': URA.car (t:=Mem1._memRA)))) (GRA.embed ((b, ofs) |-> [v])).
-      { rewrite ! GRA.embed_add. eapply GRA.embed_updatable.
-        clear - VALID WF0. clear VALID.
-        Local Transparent URA.add GRA.to_URA points_to URA.wf URA.unit.
-        eapply URA.auth_update; et.
-        rr. ii. destruct H; clear H. (*** FIXME: des runs infloop ***)
-        des. subst. esplits; et.
-        subst mem_src'. do 2 (apply func_ext; i). specialize (H0 x x0). specialize (WF0 x x0). ss.
-        des_ifs; bsimpl; des; des_sumbool; ss; subst;
-          try rewrite Z.leb_le in *; try rewrite Z.leb_gt in *; try rewrite Z.ltb_lt in *; try rewrite Z.ltb_ge in *;
-            try rewrite Z.sub_diag in *; try lia; ss.
-        Local Opaque URA.add GRA.to_URA points_to URA.wf URA.unit.
+      eapply own_upd in SIM; cycle 1; [|rewrite intro_iHyp in SIM; iMod SIM].
+      { eapply GRA.embed_updatable. eapply URA.auth_update with (a':=mem_src1) (b':=_points_to (b, ofs) [v1]); et.
+        clear - wf WF'. ii. des. subst. esplits; et.
+        do 2 ur in WF'. do 2 spc WF'.
+        subst mem_src1. ss. des_ifs; bsimpl; des; des_sumbool; ss.
+        do 2 ur. do 2 (apply func_ext; i). des_ifs.
+        - bsimpl; des; des_sumbool; subst. rewrite _points_to_hit. admit "ez".
+        - bsimpl; des; des_sumbool; rewrite ! _points_to_miss; et.
       }
-      { splits; eauto. }
-      { unfold wf. esplits; eauto. esplits; ss; et. des_ifs.
-        - bsimpl; des; des_sumbool; ss; subst. unfold mem_src'. des_ifs; bsimpl; des; des_sumbool; ss. econs; et.
-        - unfold mem_src'. des_ifs. bsimpl; des; des_sumbool; subst; ss.
+      rewrite <- GRA.embed_add in SIM. rewrite own_sep in SIM. iDestruct SIM. fold (points_to (b,ofs) [v1]) in A0.
+      force_l. eexists.
+      hret_tac SIM A0.
+      { split; [|refl]; iRefresh. ss. }
+      { ss. esplits; eauto.
+        - eexists; iRefresh. iSplitP; ss; et. ii. des_ifs.
+          + bsimpl; des; des_sumbool; subst. do 2 spc A. rewrite Heq in *. rewrite T in *.
+            unfold mem_src1. rewrite ! dec_true; ss. econs.
+          + erewrite f_equal; [apply A|]. unfold mem_src1. des_ifs. bsimpl; des; des_sumbool; subst; ss.
+        - ii. ss. des_ifs.
+          + bsimpl; des; des_sumbool; subst. eapply WFTGT; et.
+          + eapply WFTGT; et.
       }
     }
     econs; ss.
-    { unfold cmpF. init. harg_tac. unfold interp_hCallE_tgt, APC. steps.
-      destruct PRE as [[? []] ?]. subst.
-      set (resource := c).
-      assert (VALIDPTR: forall b ofs v (WF: URA.wf ((URA.black (mem_src: URA.car (t:=Mem1._memRA))) ⋅ ((b, ofs) |-> [v]))),
+    { unfold cmpF. init.
+      harg_tac. des_ifs_safe. des. repeat rewrite URA.unit_idl in *. repeat rewrite URA.unit_id in *.
+      iRefresh. do 2 iDestruct SIM. iPure A. do 2 iDestruct PRE. iPure A0. clarify.
+      rename x into mem_src0.
+      (* assert(T: mem_src0 b ofs = URA.of_RA.just (Some v)). *)
+      (* { clear - WF. *)
+      (*   apply GRA.embed_wf in WF. des; ss. eapply URA.auth_included in WF. des. *)
+      (*   eapply pw_extends in WF. eapply pw_extends in WF. rewrite _points_to_hit in WF. *)
+      (*   des; ss. *)
+      (*   admit "ez". *)
+      (* } *)
+      assert (VALIDPTR: forall b ofs v (WF: URA.wf ((URA.black (mem_src0: URA.car (t:=Mem1._memRA))) ⋅ ((b, ofs) |-> [v]))),
                  Mem.valid_ptr mem_tgt b ofs = true).
-      { clear - SIM. i. cut (mem_src b ofs = inl (Some v)).
+      { clear - A. i. cut (mem_src0 b ofs = Some v).
         - i. unfold Mem.valid_ptr.
-          specialize (SIM b ofs). rewrite H in *. inv SIM. ss.
-        - Local Transparent points_to URA.add URA.wf URA.unit.
-          ss. des. specialize (WF0 b ofs). r in WF. des; clarify. ss.
-          des_ifs; bsimpl; des; des_sumbool; ss; subst;
-            try rewrite Z.leb_le in *; try rewrite Z.leb_gt in *; try rewrite Z.ltb_lt in *; try rewrite Z.ltb_ge in *;
-              try rewrite Z.sub_diag in *; try lia; ss.
-          Local Opaque URA.add GRA.to_URA points_to URA.wf URA.unit.
+          specialize (A b ofs). rewrite H in *. inv A. ss.
+        - clear - WF.
+          eapply URA.auth_included in WF. des.
+          eapply pw_extends in WF. eapply pw_extends in WF. rewrite _points_to_hit in WF.
+          des; ss.
+          admit "ez".
       }
-      force_l. exists 0. steps. force_l. exists (if b then Vint 1 else Vint 0). des; clarify.
-      - anytac. ss. steps.
-        rewrite URA.unit_idl in *. rewrite GRA.embed_add in *. apply_all_once GRA.embed_wf. des.
-        erewrite VALIDPTR; cycle 1.
-        { instantiate (1:=v). eapply VALID. }
-        steps. hret_tac (GRA.embed (URA.black (mem_src: URA.car (t:=Mem1._memRA)))) resource; ss.
-        esplits; eauto.
-      - anytac. ss. steps.
-        rewrite URA.unit_idl in *. rewrite GRA.embed_add in *. apply_all_once GRA.embed_wf. des.
-        erewrite VALIDPTR; cycle 1.
-        { instantiate (1:=v). eapply VALID. }
-        steps. hret_tac (GRA.embed (URA.black (mem_src: URA.car (t:=Mem1._memRA)))) resource; ss.
-        esplits; eauto.
-      - anytac. ss. steps.
-        rewrite URA.unit_idl in *. repeat rewrite GRA.embed_add in *. apply_all_once GRA.embed_wf. des.
-        erewrite VALIDPTR; cycle 1.
-        { instantiate (1:=v0). clear - VALID.
-          eapply URA.wf_mon. erewrite <- URA.add_assoc. eapply VALID. }
-        erewrite VALIDPTR; cycle 1.
-        { instantiate (1:=v1). clear - VALID.
-          eapply URA.wf_mon. erewrite <- URA.add_assoc.
-          erewrite URA.add_comm with (a:=(b1, ofs1) |-> [v1]). eapply VALID. }
-        ss. destruct (dec b0 b1); cycle 1.
-        { ss. steps. hret_tac (GRA.embed (URA.black (mem_src: URA.car (t:=Mem1._memRA)))) resource; ss.
-          esplits; eauto. }
-        destruct (dec ofs0 ofs1); cycle 1.
-        { ss. steps. hret_tac (GRA.embed (URA.black (mem_src: URA.car (t:=Mem1._memRA)))) resource; ss.
-          esplits; eauto. }
-        subst. exfalso.
-        erewrite URA.add_comm in VALID. eapply URA.wf_mon in VALID.
-        Local Transparent points_to URA.add URA.wf URA.unit.
-        ss. specialize (VALID b1 ofs1).
-        destruct (dec b1 b1); ss. erewrite Z.leb_refl in *. ss.
-        replace (ofs1 <? ofs1 + 1)%Z with true in *; ss.
-        clear. symmetry. eapply Z.ltb_lt. lia.
-        Local Opaque URA.add GRA.to_URA points_to URA.wf URA.unit.
-      - anytac. ss. steps.
-        rewrite URA.unit_idl in *. rewrite GRA.embed_add in *. apply_all_once GRA.embed_wf. des.
-        erewrite VALIDPTR; cycle 1.
-        { instantiate (1:=v). eapply VALID. }
-        ss. destruct (dec b0 b0); ss. destruct (dec ofs ofs); ss. steps.
-        hret_tac (GRA.embed (URA.black (mem_src: URA.car (t:=Mem1._memRA)))) resource; ss.
-        esplits; eauto.
-      - anytac. ss. steps. rewrite URA.unit_idl in *.
-        hret_tac (GRA.embed (URA.black (mem_src: URA.car (t:=Mem1._memRA)))) resource; ss.
-        esplits; eauto.
+      steps. rewrite Any.upcast_downcast in *. steps.
+      unfold interp_hCallE_tgt, APC. steps. (********** TODO: never unfold it, make a lemma ******************)
+      force_l. exists 0. steps.
+      Ltac iDestruct H :=
+        match type of H with
+        | iHyp (Exists _, _) _ => destruct H as [? H]; iRefresh
+        | iHyp (_ ** _) _ =>
+          let name0 := fresh "A" in
+          apply sepconj_split in H as [? [? [H [name0 ?]]]]; subst; iRefresh
+        | iHyp (_ ∨ _) _ =>
+          let name0 := fresh "A" in
+          destruct H as [H|name0]; iRefresh
+        end.
+      iMerge SIM A1. rewrite <- own_sep in SIM. iOwnWf SIM. rewrite own_sep in SIM. iDestruct SIM.
+      iDestruct PRE; cycle 1.
+      { iPure A1. des; subst. apply Any.upcast_inj in A1. des; clarify. steps. force_l. eexists. hret_tac SIM A0.
+        { split; [iRefresh|refl]. iSplitP; ss. }
+        { ss. esplits; et. eexists; iRefresh. iSplitP; ss; et. }
+      }
+      iDestruct PRE; cycle 1.
+      { repeat iDestruct A1; subst. iPure A1. iPure A2. iPure A3. subst. apply Any.upcast_inj in A1. des; clarify. steps.
+        rewrite GRA.embed_add in WF. eapply GRA.embed_wf in WF; des.
+        erewrite VALIDPTR; et. ss. rewrite ! dec_true; ss. steps.
+        force_l. eexists. hret_tac SIM A0.
+        { split; [iRefresh|refl]. iSplitP; ss. }
+        { ss. esplits; et. eexists; iRefresh. iSplitP; ss; et. }
+      }
+      iDestruct PRE; cycle 1.
+      { repeat iDestruct A1; subst. iPure A1. iPure A2. iPure A3. subst. apply Any.upcast_inj in A1. des; clarify. steps.
+        rewrite ! GRA.embed_add in WF. eapply GRA.embed_wf in WF; des.
+        erewrite VALIDPTR; et; cycle 1.
+        { rewrite URA.add_assoc in WF. eapply URA.wf_mon in WF; et. }
+        erewrite VALIDPTR; et; cycle 1.
+        { rewrite URA.add_comm with (a:=(x6, x7) |-> [x8]) in WF. rewrite URA.add_assoc in WF. eapply URA.wf_mon in WF; et. }
+        rewrite URA.add_comm in WF. eapply URA.wf_mon in WF. ur in WF; ss.
+        replace (dec x6 x9 && dec x7 x10) with false; cycle 1.
+        { clear - WF.
+          assert(NEQ: x6 <> x9 \/ x7 <> x10).
+          { admit "ez". }
+          des; try (by rewrite dec_false; ss). rewrite dec_false with (x0:=x7); ss. rewrite andb_false_r; ss.
+        }
+        steps.
+        force_l. eexists. hret_tac SIM A0.
+        { split; [iRefresh|refl]. iSplitP; ss. }
+        { ss. esplits; et. eexists; iRefresh. iSplitP; ss; et. }
+      }
+      iDestruct PRE; cycle 1.
+      { repeat iDestruct A1; subst. iPure A1. iPure A2. iPure A3. subst. apply Any.upcast_inj in A1. des; clarify. steps.
+        rewrite GRA.embed_add in WF. eapply GRA.embed_wf in WF; des.
+        erewrite VALIDPTR; et. ss. steps.
+        force_l. eexists. hret_tac SIM A0.
+        { split; [iRefresh|refl]. iSplitP; ss. }
+        { ss. esplits; et. eexists; iRefresh. iSplitP; ss; et. }
+      }
+      iDestruct PRE; cycle 1.
+      { repeat iDestruct PRE; subst. iPure A1. iPure A2. iPure PRE. subst. apply Any.upcast_inj in PRE. des; clarify. steps.
+        rewrite GRA.embed_add in WF. eapply GRA.embed_wf in WF; des.
+        erewrite VALIDPTR; et. ss. steps.
+        force_l. eexists. hret_tac SIM A0.
+        { split; [iRefresh|refl]. iSplitP; ss. }
+        { ss. esplits; et. eexists; iRefresh. iSplitP; ss; et. }
+      }
     }
   Qed.
 
